Fixed padding Makefile target

examples/crypto/Padding.MAC2.fst
@@ -2,49 +2,48 @@ module Padding.MAC2
 
 open FStar.Seq
 open FStar.SeqProperties
+
 open Padding.Pad
+open Padding.BMAC
 
 type text2 = b:bytes { length b <=  blocksize }
 
 let keysize = 2 * BMAC.keysize
 let macsize = BMAC.macsize
+
 type key = | Keys: k0:BMAC.key -> k1:BMAC.key -> key
 type tag = BMAC.tag
 
-opaque type bspec0 (spec: (text2 -> Type)) (b:block) =
-  (forall (t:text). b = encode t ==> spec t)
+opaque type bspec0 (spec:text2 -> Type) (b:block) =
+  forall (t:text). b = encode t ==> spec t
 
-opaque type bspec1 (spec: (text2 -> Type)) (b:block) =
+opaque type bspec1 (spec:text2 -> Type) (b:block) =
   spec b
 
-opaque type key_prop : key -> text2 -> Type
+opaque new type key_prop: key -> text2 -> Type
 
-type pkey (p:(text2 -> Type)) =
+type pkey (p:text2 -> Type) =
   k:key{ key_prop k == p
-      /\ BMAC.key_prop (Keys.k0 k) == bspec0 p
-      /\ BMAC.key_prop (Keys.k1 k) == bspec1 p }
+      /\ (forall b. BMAC.key_prop (Keys.k0 k) b == bspec0 p b) 
+      /\ (forall b. BMAC.key_prop (Keys.k1 k) b == bspec1 p b) }
 
 val keygen: p:(text2 -> Type) -> pkey p
-val mac:    p:(text2 -> Type) -> k:pkey p -> t:text2{p  t} -> tag
+val mac:    p:(text2 -> Type) -> k:pkey p -> t:text2{p t} -> tag
 val verify: p:(text2 -> Type) -> k:pkey p -> t:text2 -> tag -> b:bool{b ==> p t}
 
-(* not verified yet: *)
-let keygen (spec: text2 -> Type) =
-  let k0 = BMAC.keygen (bspec0 spec) in
-  let k1 = BMAC.keygen (bspec1 spec) in
+let keygen (p:text2 -> Type) =
+  let k0 = BMAC.keygen (bspec0 p) in
+  let k1 = BMAC.keygen p in
   let k = Keys k0 k1 in
-  assert (BMAC.key_prop k0 == bspec0 spec);
-  assert (BMAC.key_prop k1 == bspec1 spec);
-  assume (key_prop k == spec);
+  assume (key_prop k == p);
   k
 
-
-let mac (Keys k0 k1) t =
+let mac (p:text2 -> Type) k t =
   if length t < blocksize
-  then BMAC.mac k0 (encode t)
-  else BMAC.mac k1 t
+  then BMAC.mac k.k0 (encode t)
+  else BMAC.mac k.k1 t
 
-let verify (Keys k0 k1) t tag =
+let verify (p:text2 -> Type) k t tag =
   if length t < blocksize
-  then BMAC.verify k0 (encode t) tag
-  else BMAC.verify k1 t tag
+  then BMAC.verify k.k0 (encode t) tag
+  else BMAC.verify k.k1 t tag
